size classes metaprogrammation: improve and clean
- list of size classes moved to config file,
behind an interface
- metaprogrammation requires breaking this
abstraction: corresponding code is thus moved
from Main.fst to Main.Meta.fst
overall, some cleaning, recompilation when
editing size classes is way faster
TODO: some remaining assumes/small admits

src/Config.fst
@@ -7,21 +7,55 @@ open FStar.Mul
 module A = Steel.Array
 let _ : squash (US.fits_u64)
   = A.intro_fits_u64 ()
+
+let _ : squash (US.fits_u32)
+  = A.intro_fits_u32 ()
+
 let _ : squash (UP.fits (FStar.Int.max_int 64))
   = A.intro_fits_ptrdiff64 ()
+
+let sc_list = [
+    16ul; 32ul; 64ul;
+    128ul; 256ul; 512ul;
+    1024ul; 2048ul; 4096ul
+  ]
+
+module U16 = FStar.UInt16
+module U32 = FStar.UInt32
+
+//DO NOT EDIT, edit sc_list instead
+let nb_size_classes
+  =
+  assert_norm (L.length sc_list < U32.n);
+  [@inline_let] let l = normalize_term (L.length sc_list) in
+  normalize_term_spec (L.length sc_list);
+  assert (l == L.length sc_list);
+  [@inline_let] let l_as_u32 = normalize_term (U32.uint_to_t l) in
+  normalize_term_spec (U32.uint_to_t l);
+  assert (U32.v l_as_u32 == L.length sc_list);
+  // do not normalize cast to size_t,
+  // as it is internally represented uint64_t
+  // and yields a type mismatch
+  US.of_u32 l_as_u32
+
+let nb_arenas = 4sz
 
 inline_for_extraction noextract
 let metadata_max' = 1048576UL
 
+//DO NOT EDIT, edit metadata_max' instead
 let metadata_max =
+  admit ();
+  assert_norm (U32.v page_size * U64.v metadata_max' * US.v nb_size_classes * US.v nb_arenas < U64.n);
   US.fits_u64_implies_fits (U32.v page_size * U64.v metadata_max' * US.v nb_size_classes * US.v nb_arenas);
   US.fits_u64_implies_fits (U64.v metadata_max');
   US.of_u64 metadata_max'
 
+//DO NOT EDIT
 let metadata_max_up_fits _ = ()
-
+//DO NOT EDIT
 let alg_null = US.v metadata_max + 1
-
+//DO NOT EDIT
 let alg_null_sizet = US.add metadata_max 1sz
 
 // guard pages
