src/Utils2.fsti
@@ -24,32 +24,6 @@ unfold let same_base_array (#a: Type) (arr1 arr2: array a)
 
 unfold let slab_metadata = r:array U64.t{A.length r = 4}
 
-noextract
-let min_sc = 64
-noextract
-let max_sc = U32.v page_size
-
-// TODO: this could be improved
-// currently does not support size classes
-// such that:
-// - sc < 64, thus nb_slot sc > 64
-// and
-// - (nb_slots sc) % 64 <> 0
-// this allows to only have a particular mechanism
-// for the first u64 of the bitmap
-// note: this mechanism does not rely on any loop!
-let sc = x:U32.t{
-  (
-    U32.eq x 16ul \/
-    U32.eq x 32ul \/
-    (min_sc <= U32.v x /\ U32.v x <= max_sc)
-  ) /\
-  // https://www.intel.com/content/dam/develop/external/us/en/documents/mpx-linux64-abi.pdf
-  // allocated arrays should have alignment of at least 16 bytes,
-  // allowing use of SSE instructions
-  (U32.v x % 16 == 0)
-}
-
 // abstract property that the underlying pointer is 16-bytes aligned
 //assume
 val array_u8_proper_alignment (arr: array U8.t): prop
