src/Main.Meta.fsti
@@ -1,0 +1,156 @@
+module Main.Meta
+
+module U8 = FStar.UInt8
+module U32 = FStar.UInt32
+module U64 = FStar.UInt64
+module US = FStar.SizeT
+module UP = FStar.PtrdiffT
+module G = FStar.Ghost
+
+open Steel.Effect.Atomic
+open Steel.Effect
+open Steel.Array
+module A = Steel.Array
+module AL = ArrayList
+module SAA = Steel.ArrayArith
+module L = Steel.SpinLock
+
+open Prelude
+open FStar.Mul
+open SlabsCommon
+open SizeClass
+open Main
+open Mman
+open Config
+open Utils2
+open NullOrVarray
+open Main
+open ROArray
+
+/// The total number of size classes in the allocator, across all arenas.
+/// Used as an abbreviation for specification purposes
+inline_for_extraction noextract
+val total_nb_sc: nat
+
+/// This gathers all the data for small allocations.
+/// In particular, it contains an array with all size_classes data,
+/// as well as the slab_region containing the actual memory
+noeq
+type size_classes_all =
+  { size_classes : sc:array size_class{length sc == total_nb_sc}; // The array of size_classes
+    sizes : sz:array sc{length sz == total_nb_sc}; // An array of the sizes of [size_classes]
+    g_size_classes: Ghost.erased (Seq.lseq size_class (length size_classes)); // The ghost representation of size_classes
+    g_sizes: Ghost.erased (Seq.lseq sc (length sizes)); // The ghost representation of sizes
+    ro_perm: ro_array size_classes g_size_classes; // The read-only permission on size_classes
+    ro_sizes: ro_array sizes g_sizes;
+    slab_region: arr:array U8.t{ // The region of memory handled by this size class
+      synced_sizes total_nb_sc g_sizes g_size_classes /\
+      A.length arr == US.v slab_region_size /\
+      (forall (i:nat{i < Seq.length g_size_classes}).
+        size_class_pred arr (Seq.index g_size_classes i) i)
+    }
+  }
+
+val sc_all : size_classes_all
+
+module T = FStar.Tactics
+
+/// A variant of the normalization, with a zeta full to reduce under
+/// matches (and if/then/else). To use with care, as zeta_full can
+/// loop and lead to stack overflows
+noextract
+let norm_full () : T.Tac unit =
+  T.norm [zeta_full; iota; primops; delta_attr [`%reduce_attr]];
+  T.trefl ()
+
+[@@ T.postprocess_with norm_full]
+val slab_malloc
+  (arena_id: US.t{US.v arena_id < US.v nb_arenas})
+  (bytes: U32.t)
+  : Steel (array U8.t)
+  emp
+  (fun r -> null_or_varray r)
+  (requires fun _ -> True)
+  (ensures fun _ r h1 ->
+    let s : t_of (null_or_varray r)
+      = h1 (null_or_varray r) in
+    not (is_null r) ==> (
+      A.length r >= U32.v bytes /\
+      array_u8_proper_alignment r /\
+      Seq.length s >= 2 /\
+      (enable_slab_canaries_malloc ==>
+        Seq.index s (A.length r - 2) == slab_canaries_magic1 /\
+        Seq.index s (A.length r - 1) == slab_canaries_magic2
+      )
+    )
+  )
+
+[@@ T.postprocess_with norm_full]
+val slab_aligned_alloc (arena_id:US.t{US.v arena_id < US.v nb_arenas}) (alignment:U32.t) (bytes:U32.t)
+  : Steel (array U8.t)
+  emp
+  (fun r -> null_or_varray r)
+  (requires fun _ -> True)
+  (ensures fun _ r h1 ->
+    let s : t_of (null_or_varray r)
+      = h1 (null_or_varray r) in
+    not (is_null r) ==> (
+      A.length r >= U32.v bytes /\
+      array_u8_proper_alignment r /\
+      Seq.length s >= 2 /\
+      (enable_slab_canaries_malloc ==>
+        Seq.index s (A.length r - 2) == slab_canaries_magic1 /\
+        Seq.index s (A.length r - 1) == slab_canaries_magic2
+      )
+    )
+  )
+
+val within_size_classes_pred (ptr:A.array U8.t) : prop
+
+val slab_getsize (ptr: array U8.t)
+  : Steel US.t
+  (A.varray ptr `star` A.varray (A.split_l sc_all.slab_region 0sz))
+  (fun _ ->
+   A.varray ptr `star` A.varray (A.split_l sc_all.slab_region 0sz))
+  (requires fun _ ->
+    within_size_classes_pred ptr /\
+    SAA.within_bounds
+      (A.split_l (G.reveal sc_all.slab_region) 0sz)
+      ptr
+      (A.split_r (G.reveal sc_all.slab_region) slab_region_size)
+  )
+  (ensures fun h0 r h1 ->
+    A.asel ptr h1 == A.asel ptr h0 /\
+    (r <> 0sz ==>
+      (enable_slab_canaries_malloc ==>
+        A.length ptr == US.v r + 2
+      ) /\
+      (not enable_slab_canaries_malloc ==>
+        A.length ptr == US.v r
+      )
+    )
+  )
+
+val slab_free (ptr:array U8.t)
+  : Steel bool
+  (A.varray ptr `star`
+    A.varray (A.split_l sc_all.slab_region 0sz))
+  (fun b ->
+    (if b then emp else A.varray ptr) `star`
+    A.varray (A.split_l sc_all.slab_region 0sz))
+  (requires fun _ ->
+    within_size_classes_pred ptr /\
+    SAA.within_bounds
+      (A.split_l (G.reveal sc_all.slab_region) 0sz)
+      ptr
+      (A.split_r (G.reveal sc_all.slab_region) slab_region_size)
+  )
+  (ensures fun h0 r _ ->
+    let s = A.asel ptr h0 in
+    enable_slab_canaries_free ==>
+      (r ==>
+        A.length ptr >= 2 /\
+        Seq.index s (A.length ptr - 2) == slab_canaries_magic1 /\
+        Seq.index s (A.length ptr - 1) == slab_canaries_magic2
+      )
+  )
